pulse/examples/dsls/mini_steel/Pulse.Steel.Wrapper.fsti
@@ -259,3 +259,9 @@ val elim_exists (#a:Type) (p:a -> vprop)
 
 val intro_exists (#a:Type) (p:a -> vprop) (e:a)
   : stt_ghost unit emp_inames (p e) (fun _ -> exists_ p)
+
+val while_loop
+  (inv:bool -> vprop)
+  (cond:stt bool (exists_ inv) inv)
+  (body:stt unit (inv true) (fun _ -> exists_ inv))
+  : stt unit (exists_ inv) (fun _ -> inv false)
